rename Context to Env

Juvix/Core/Main/Language/Value.lean
@@ -7,9 +7,9 @@ inductive Value : Type where
   | unit : Value
   | const : Constant → Value
   | constr_app : (constr : Name) → (args_rev : List Value) → Value
-  | closure : (ctx : List Value) → (value : Expr) → Value
+  | closure : (env : List Value) → (value : Expr) → Value
   deriving Inhabited
 
-abbrev Context : Type := List Value
+abbrev Env : Type := List Value
 
 end Juvix.Core.Main
