Juvix/Core/Main/Semantics/Eval.lean
@@ -11,57 +11,57 @@ def eval_binop_int (op : BinaryOp) (i₁ i₂ : Int) : Int :=
   | BinaryOp.mul_int => i₁ * i₂
   | BinaryOp.div_int => i₁ / i₂
 
-inductive Eval (P : Program) : Context → Expr → Value → Prop where
-  | eval_var {ctx idx val} :
-    ctx.get? idx = some val →
-    Eval P ctx (Expr.var idx) val
-  | eval_ident {ctx name expr val} :
+inductive Eval (P : Program) : Env → Expr → Value → Prop where
+  | eval_var {env idx val} :
+    env.get? idx = some val →
+    Eval P env (Expr.var idx) val
+  | eval_ident {env name expr val} :
     P.defs.find? name = some expr →
     Eval P [] expr val →
-    Eval P ctx (Expr.ident name) val
-  | eval_const {ctx c} :
-    Eval P ctx (Expr.const c) (Value.const c)
-  | eval_app {ctx ctx' f body arg val val'} :
-    Eval P ctx f (Value.closure ctx' body) →
-    Eval P ctx arg val →
-    Eval P (val :: ctx') body val' →
-    Eval P ctx (Expr.app f arg) val'
-  | eval_constr_app {ctx ctr ctr_name ctr_args_rev arg val} :
-    Eval P ctx ctr (Value.constr_app ctr_name ctr_args_rev) →
-    Eval P ctx arg val →
-    Eval P ctx (Expr.constr_app ctr arg) (Value.constr_app ctr_name (val :: ctr_args_rev))
-  | eval_binop {ctx op arg₁ arg₂ val₁ val₂} :
-    Eval P ctx arg₁ (Value.const (Constant.int val₁)) →
-    Eval P ctx arg₂ (Value.const (Constant.int val₂)) →
-    Eval P ctx (Expr.binop op arg₁ arg₂) (Value.const (Constant.int (eval_binop_int op val₁ val₂)))
-  | eval_lambda {ctx body} :
-    Eval P ctx (Expr.lambda body) (Value.closure ctx body)
-  | eval_save {ctx value body val val'} :
-    Eval P ctx value val →
-    Eval P (val :: ctx) body val' →
-    Eval P ctx (Expr.save value body) val'
-  | eval_branch_matches {ctx name args_rev body val} :
-    Eval P (args_rev ++ ctx) body val →
-    Eval P (Value.constr_app name args_rev :: ctx) (Expr.branch name body _) val
-  | eval_branch_fails {ctx name name' next val} :
+    Eval P env (Expr.ident name) val
+  | eval_const {env c} :
+    Eval P env (Expr.const c) (Value.const c)
+  | eval_app {env env' f body arg val val'} :
+    Eval P env f (Value.closure env' body) →
+    Eval P env arg val →
+    Eval P (val :: env') body val' →
+    Eval P env (Expr.app f arg) val'
+  | eval_constr_app {env ctr ctr_name ctr_args_rev arg val} :
+    Eval P env ctr (Value.constr_app ctr_name ctr_args_rev) →
+    Eval P env arg val →
+    Eval P env (Expr.constr_app ctr arg) (Value.constr_app ctr_name (val :: ctr_args_rev))
+  | eval_binop {env op arg₁ arg₂ val₁ val₂} :
+    Eval P env arg₁ (Value.const (Constant.int val₁)) →
+    Eval P env arg₂ (Value.const (Constant.int val₂)) →
+    Eval P env (Expr.binop op arg₁ arg₂) (Value.const (Constant.int (eval_binop_int op val₁ val₂)))
+  | eval_lambda {env body} :
+    Eval P env (Expr.lambda body) (Value.closure env body)
+  | eval_save {env value body val val'} :
+    Eval P env value val →
+    Eval P (val :: env) body val' →
+    Eval P env (Expr.save value body) val'
+  | eval_branch_matches {env name args_rev body val} :
+    Eval P (args_rev ++ env) body val →
+    Eval P (Value.constr_app name args_rev :: env) (Expr.branch name body _) val
+  | eval_branch_fails {env name name' next val} :
     name ≠ name' →
-    Eval P ctx next val →
-    Eval P (Value.constr_app name _ :: ctx) (Expr.branch name' _ next) val
-  | eval_default {ctx body val} :
-    Eval P ctx body val →
-    Eval P (_ :: ctx) (Expr.default body) val
-  | eval_unit {ctx} :
-    Eval P ctx Expr.unit Value.unit
+    Eval P env next val →
+    Eval P (Value.constr_app name _ :: env) (Expr.branch name' _ next) val
+  | eval_default {env body val} :
+    Eval P env body val →
+    Eval P (_ :: env) (Expr.default body) val
+  | eval_unit {env} :
+    Eval P env Expr.unit Value.unit
 
-notation "⟨" P "⟩ " ctx " ⊢ " e " ↦ " v:40 => Eval P ctx e v
+notation "⟨" P "⟩ " env " ⊢ " e " ↦ " v:40 => Eval P env e v
 
-def Terminating (P : Program) (ctx : Context) (e : Expr) : Prop :=
-  ∃ v, ⟨P⟩ ctx ⊢ e ↦ v
+def Terminating (P : Program) (env : Env) (e : Expr) : Prop :=
+  ∃ v, ⟨P⟩ env ⊢ e ↦ v
 
-notation "⟨" P "⟩ " ctx " ⊢ " e:40 " ↓" => Terminating P ctx e
+notation "⟨" P "⟩ " env " ⊢ " e:40 " ↓" => Terminating P env e
 
 -- The evaluation relation is deterministic.
-theorem Eval.deterministic {P ctx e v₁ v₂} (h₁ : ⟨P⟩ ctx ⊢ e ↦ v₁) (h₂ : ⟨P⟩ ctx ⊢ e ↦ v₂) : v₁ = v₂ := by
+theorem Eval.deterministic {P env e v₁ v₂} (h₁ : ⟨P⟩ env ⊢ e ↦ v₁) (h₂ : ⟨P⟩ env ⊢ e ↦ v₂) : v₁ = v₂ := by
   induction h₁ generalizing v₂ with
   | eval_var =>
     cases h₂ <;> cc
